theories/WPTactics.v
@@ -258,7 +258,7 @@ Ltac xseq_pre tt :=
   | (Wpgen_seq _ _) => idtac 
   end.
 
-Definition xseq_lemma := @mkLocal_erase.
+Definition xseq_lemma := @MkStruct_erase.
 
 Ltac xseq_core tt :=
   xseq_pre tt;
@@ -274,9 +274,9 @@ Tactic Notation "xseq" :=
 Lemma xlet_lemma : forall A1 (EA1:Enc A1) H `{EA:Enc A} (Q:A->hprop) (F1:Formula) (F2of:forall `{EA1:Enc A2},A2->Formula),
   H ==> ^F1 (fun (X:A1) => ^(F2of X) Q) -> 
   H ==> ^(Wpgen_let F1 (@F2of)) Q.
-Proof using. introv M. applys mkLocal_erase. hsimpl* A1 EA1. Qed.
+Proof using. introv M. applys MkStruct_erase. hsimpl* A1 EA1. Qed.
 
-Definition xlet_typed_lemma := @mkLocal_erase.
+Definition xlet_typed_lemma := @MkStruct_erase.
 
 Ltac xlet_poly tt :=
   notypeclasses refine (xlet_lemma _ _ _ _ _).
@@ -362,7 +362,7 @@ Lemma xapp_lemma : forall A `{EA:Enc A} (Q1:A->hprop) t H1 H Q,
   H ==> H1 \* (Q1 \--* protect Q) ->
   H ==> ^(Wpgen_app t) Q.
 Proof using.
-  introv M1 M2. applys mkLocal_erase.
+  introv M1 M2. applys MkStruct_erase.
   hchanges (rm M2).
   rewrite <- Triple_eq_himpl_Wp.
   applys* Triple_ramified_frame.
@@ -508,14 +508,14 @@ Lemma xval_lemma : forall `{EA:Enc A} (V:A) v H (Q:A->hprop),
   v = ``V ->
   H ==> Q V ->
   H ==> ^(Wpgen_val v) Q.
-Proof using. introv E N. subst. applys mkLocal_erase. hsimpl~ V. Qed.
+Proof using. introv E N. subst. applys MkStruct_erase. hsimpl~ V. Qed.
 
 (* NEEDED? *)
 Lemma xval_lemma_val : forall `{EA:Enc A} (V:A) v H (Q:val->hprop),
   v = ``V ->
   H ==> Q (``V) ->
   H ==> ^(Wpgen_val v) Q.
-Proof using. introv E N. subst. applys mkLocal_erase. hsimpl~ (``V). Qed.
+Proof using. introv E N. subst. applys MkStruct_erase. hsimpl~ (``V). Qed.
 
 (* [xval_pre tt] automatically performs the necessary 
    [xlet], [xseq] and [xcast], then checks that the goal 
@@ -563,13 +563,13 @@ Lemma xifval_lemma : forall `{EA:Enc A} b H (Q:A->hprop) (F1 F2:Formula),
   (b = true -> H ==> ^F1 Q) ->
   (b = false -> H ==> ^F2 Q) ->
   H ==> ^(Wpgen_if_bool b F1 F2) Q.
-Proof using. introv E N. applys mkLocal_erase. case_if*. Qed.
+Proof using. introv E N. applys MkStruct_erase. case_if*. Qed.
 
 Lemma xifval_lemma_isTrue : forall `{EA:Enc A} (P:Prop) H (Q:A->hprop) (F1 F2:Formula),
   (P -> H ==> ^F1 Q) ->
   (~ P -> H ==> ^F2 Q) ->
   H ==> ^(Wpgen_if_bool (isTrue P) F1 F2) Q.
-Proof using. introv E N. applys mkLocal_erase. case_if*. Qed.
+Proof using. introv E N. applys MkStruct_erase. case_if*. Qed.
 
 Ltac xif_core tt :=
   first [ applys @xifval_lemma_isTrue
@@ -593,7 +593,7 @@ Lemma xcase_lemma : forall F1 (P:Prop) F2 H `{EA:Enc A} (Q:A->hprop),
   (P -> H ==> ^F2 Q) ->
   H ==> ^(Wpgen_case F1 P F2) Q.
 Proof using. 
-  introv M1 M2. apply mkLocal_erase. applys himpl_hand_r. 
+  introv M1 M2. apply MkStruct_erase. applys himpl_hand_r. 
   { auto. }
   { applys* hwand_hpure_r_intro. }
 Qed.
